Iterator/Combinators/MonadLift.lean
@@ -12,10 +12,10 @@ variable {α : Type w} {m : Type w → Type w'} {n : Type w → Type w''} {β : 
     [Monad m] [Monad n]
 
 structure MonadLiftIterator (α : Type w) (m : Type w → Type w') {β : Type v} [Iterator α m β] (n : Type w → Type w'') [MonadLiftT m n] where
-  inner : Iter (α := α) m β
+  inner : IterM (α := α) m β
 
-inductive MonadLiftIterator.PlausibleStep {_ : Iterator α m β} {_ : MonadLiftT m n} (it : Iter (α := MonadLiftIterator α m n) n β) :
-    IterStep (Iter (α := MonadLiftIterator α m n) n β) β → Prop where
+inductive MonadLiftIterator.PlausibleStep {_ : Iterator α m β} {_ : MonadLiftT m n} (it : IterM (α := MonadLiftIterator α m n) n β) :
+    IterStep (IterM (α := MonadLiftIterator α m n) n β) β → Prop where
   | yield {it' out} (h : it.inner.inner.plausible_step (.yield it' out)) :
       PlausibleStep it (.yield ⟨⟨it'⟩⟩ out)
   | skip {it'} (h : it.inner.inner.plausible_step (.skip it')) :
@@ -23,7 +23,7 @@ inductive MonadLiftIterator.PlausibleStep {_ : Iterator α m β} {_ : MonadLiftT
   | done (h : it.inner.inner.plausible_step .done) :
       PlausibleStep it .done
 
-instance {_ : Iterator α m β} {_ : MonadLiftT m n} {it : Iter (α := MonadLiftIterator α m n) n β} :
+instance {_ : Iterator α m β} {_ : MonadLiftT m n} {it : IterM (α := MonadLiftIterator α m n) n β} :
     Small.{w} (Subtype <| MonadLiftIterator.PlausibleStep it) := sorry
 
 instance MonadLiftIterator.instIterator {_ : Iterator α m β} {_ : MonadLiftT m n} : Iterator (MonadLiftIterator α m n) n β where
@@ -40,7 +40,7 @@ instance MonadLiftIterator.instIteratorFor [Monad n] [Monad n'] [MonadLiftT n n'
   .defaultImplementation
 
 instance {_ : Iterator α m β} [Finite α m] {_ : MonadLiftT m n} : FinitenessRelation (MonadLiftIterator α m n) n where
-  rel := InvImage Iter.TerminationMeasures.Finite.rel fun it => it.inner.inner.finitelyManySteps
+  rel := InvImage IterM.TerminationMeasures.Finite.rel fun it => it.inner.inner.finitelyManySteps
   wf := by
     apply InvImage.wf
     exact WellFoundedRelation.wf
@@ -49,21 +49,21 @@ instance {_ : Iterator α m β} [Finite α m] {_ : MonadLiftT m n} : FinitenessR
     cases h'
     case yield it' out h =>
       cases h
-      exact Iter.TerminationMeasures.Finite.rel_of_yield ‹_›
+      exact IterM.TerminationMeasures.Finite.rel_of_yield ‹_›
     case skip it' h =>
       cases h
-      exact Iter.TerminationMeasures.Finite.rel_of_skip ‹_›
+      exact IterM.TerminationMeasures.Finite.rel_of_skip ‹_›
     case done h =>
       cases h
 
 variable (n) in
 @[always_inline, inline]
-def Iter.monadLift [Iterator α m β] {_ : MonadLiftT m n} (it : Iter (α := α) m β) :=
-  (toIter (MonadLiftIterator.mk it (m := m) (n := n)) n β : Iter n β)
+def IterM.monadLift [Iterator α m β] {_ : MonadLiftT m n} (it : IterM (α := α) m β) :=
+  (toIter (MonadLiftIterator.mk it (m := m) (n := n)) n β : IterM n β)
 
 @[always_inline, inline]
-def Iter.switchMonad {α : Type w} {m : Type w → Type w'} {n : Type w → Type w''} {β : Type v}
+def IterM.switchMonad {α : Type w} {m : Type w → Type w'} {n : Type w → Type w''} {β : Type v}
     [Monad m] [Monad n] [Iterator α m β]
-    (it : Iter (α := α) m β) (lift : ∀ {γ}, m γ → n γ) :=
+    (it : IterM (α := α) m β) (lift : ∀ {γ}, m γ → n γ) :=
   haveI : MonadLift m n := ⟨lift⟩
-  (toIter (MonadLiftIterator.mk it (m := m) (n := n)) n β : Iter n β)
+  (toIter (MonadLiftIterator.mk it (m := m) (n := n)) n β : IterM n β)
