Iterator/Combinators/Take.lean
@@ -10,14 +10,14 @@ import Iterator.Consumers.Loop
 import Iterator.HetT
 
 /-!
-This file provides the iterator combinator `Iter.take`.
+This file provides the iterator combinator `IterM.take`.
 -/
 
 variable {α : Type w} {m : Type w → Type w'} {β : Type v}
 
 structure Take (α : Type w) (m : Type w → Type w') (β : Type v) where
   remaining : Nat
-  inner : Iter (α := α) m β
+  inner : IterM (α := α) m β
 
 /--
 Given an iterator `it` and a natural number `n`, `it.take n` is an iterator that outputs
@@ -45,16 +45,16 @@ _TODO_: prove `Productive`
 This combinator incurs an additional O(1) cost with each output of `it`.
 -/
 @[inline]
-def Iter.take (n : Nat) (it : Iter (α := α) m β) :=
+def IterM.take (n : Nat) (it : IterM (α := α) m β) :=
   toIter (Take.mk n it) m β
 
-theorem Iter.take.surjective {α : Type w} {m : Type w → Type w'} {β : Type v}
-    (it : Iter (α := Take α m β) m β) :
-    ∃ (it₀ : Iter (α := α) m β) (k : Nat), it = it₀.take k := by
+theorem IterM.take.surjective {α : Type w} {m : Type w → Type w'} {β : Type v}
+    (it : IterM (α := Take α m β) m β) :
+    ∃ (it₀ : IterM (α := α) m β) (k : Nat), it = it₀.take k := by
   refine ⟨it.inner.inner, it.inner.remaining, rfl⟩
 
-inductive Take.PlausibleStep [Iterator α m β] (it : Iter (α := Take α m β) m β) :
-    (step : IterStep (Iter (α := Take α m β) m β) β) → Prop where
+inductive Take.PlausibleStep [Iterator α m β] (it : IterM (α := Take α m β) m β) :
+    (step : IterStep (IterM (α := Take α m β) m β) β) → Prop where
   | yield : ∀ {it' out k}, it.inner.inner.plausible_step (.yield it' out) →
       it.inner.remaining = k + 1 → PlausibleStep it (.yield (it'.take k) out)
   | skip : ∀ {it' k}, it.inner.inner.plausible_step (.skip it') →
@@ -63,8 +63,8 @@ inductive Take.PlausibleStep [Iterator α m β] (it : Iter (α := Take α m β) 
   | depleted : it.inner.remaining = 0 →
       PlausibleStep it .done
 
-def Take.step [Monad m] [Iterator α m β] (it : Iter (α := Take α m β) m β) :
-    HetT m (IterStep (Iter (α := Take α m β) m β) β) :=
+def Take.step [Monad m] [Iterator α m β] (it : IterM (α := Take α m β) m β) :
+    HetT m (IterStep (IterM (α := Take α m β) m β) β) :=
   match it.inner.remaining with
   | 0 => pure .done
   | k + 1 => do
@@ -73,7 +73,7 @@ def Take.step [Monad m] [Iterator α m β] (it : Iter (α := Take α m β) m β)
     | .skip it' => return .skip (it'.take (k + 1))
     | .done => return .done
 
-theorem Take.PlausibleStep.char [Monad m] [Iterator α m β] {it : Iter (α := Take α m β) m β} :
+theorem Take.PlausibleStep.char [Monad m] [Iterator α m β] {it : IterM (α := Take α m β) m β} :
     Take.PlausibleStep it = (Take.step it).property := by
   ext step
   simp only [Take.step]
@@ -84,7 +84,7 @@ theorem Take.PlausibleStep.char [Monad m] [Iterator α m β] {it : Iter (α := T
       cases h <;> (try omega; done) <;> rfl
     · rintro rfl
       exact .depleted ‹_›
-  · simp [bind, HetT.bindH, Iter.stepHet]
+  · simp [bind, HetT.bindH, IterM.stepHet]
     constructor
     · intro h
       cases h
@@ -108,7 +108,7 @@ theorem Take.PlausibleStep.char [Monad m] [Iterator α m β] {it : Iter (α := T
       · cases h
         exact .done hp
 
-instance [Iterator α m β] [Monad m] {it : Iter (α := Take α m β) m β} :
+instance [Iterator α m β] [Monad m] {it : IterM (α := Take α m β) m β} :
     Small.{w} (Subtype <| Take.PlausibleStep it) := by
   rw [Take.PlausibleStep.char]
   exact (Take.step it).small
@@ -126,15 +126,15 @@ instance Take.instIterator [Monad m] [Iterator α m β] : Iterator (Take α m β
       | .done h' => pure <| .deflate <| .done (.done h')
 
 def Take.rel (m : Type w → Type w') [Monad m] [Iterator α m β] [Productive α m] :
-    Iter (α := Take α m β) m β → Iter (α := Take α m β) m β → Prop :=
-  InvImage (Prod.Lex Nat.lt_wfRel.rel Iter.TerminationMeasures.Productive.rel)
+    IterM (α := Take α m β) m β → IterM (α := Take α m β) m β → Prop :=
+  InvImage (Prod.Lex Nat.lt_wfRel.rel IterM.TerminationMeasures.Productive.rel)
     (fun it => (it.inner.remaining, it.inner.inner.finitelyManySkips))
 
-theorem Take.rel_of_remaining [Monad m] [Iterator α m β] [Productive α m] {it it' : Iter (α := Take α m β) m β}
+theorem Take.rel_of_remaining [Monad m] [Iterator α m β] [Productive α m] {it it' : IterM (α := Take α m β) m β}
     (h : it'.inner.remaining < it.inner.remaining) : Take.rel m it' it :=
   Prod.Lex.left _ _ h
 
-theorem Take.rel_of_inner [Monad m] [Iterator α m β] [Productive α m] {remaining : Nat} {it it' : Iter (α := α) m β}
+theorem Take.rel_of_inner [Monad m] [Iterator α m β] [Productive α m] {remaining : Nat} {it it' : IterM (α := α) m β}
     (h : it'.finitelyManySkips.rel it.finitelyManySkips) :
     Take.rel m (it'.take remaining) (it.take remaining) :=
   Prod.Lex.right _ h
@@ -153,13 +153,13 @@ instance Take.instFinitenessRelation [Monad m] [Iterator α m β] [Productive α
     case yield it' out k h' h'' =>
       cases h
       apply rel_of_remaining
-      simp_all [Iter.take]
+      simp_all [IterM.take]
     case skip it' out k h' h'' =>
       cases h
-      obtain ⟨it, k, rfl⟩ := Iter.take.surjective it
+      obtain ⟨it, k, rfl⟩ := IterM.take.surjective it
       cases h''
       apply Take.rel_of_inner
-      exact Iter.TerminationMeasures.Productive.rel_of_skip h'
+      exact IterM.TerminationMeasures.Productive.rel_of_skip h'
     case done _ =>
       cases h
     case depleted _ =>
@@ -180,13 +180,13 @@ instance Take.instIteratorFor [Monad m] [Monad n] [MonadLiftT m n] [Iterator α 
     --     return match result.val with
     --     | .yield x => .yield ⟨
     --     | .done x => sorry
-    -- refine Subrelation.wf (r := InvImage Iter.TerminationMeasures.Finite.rel (fun p => (p.1).finitelyManySteps)) ?_ ?_
+    -- refine Subrelation.wf (r := InvImage IterM.TerminationMeasures.Finite.rel (fun p => (p.1).finitelyManySteps)) ?_ ?_
     -- · intro p' p h
     --   cases h
-    --   · apply Iter.plausible_successor_of_skip
+    --   · apply IterM.plausible_successor_of_skip
     --     rename_i h
     --     exact h.1
     --   · rename_i h
     --     obtain ⟨out, h, _⟩ := h -- Interesting: Moving `obtain` after `apply` leads to failure
-    --     apply Iter.plausible_successor_of_yield
+    --     apply IterM.plausible_successor_of_yield
     --     exact h
