Iterator/Lemmas/Consumer.lean
@@ -5,22 +5,22 @@ import Iterator.Producers
 
 section Consumers
 
-def Iter.induct {α m β} [Iterator α m β] [Finite α m]
-  (motive : Iter (α := α) m β → Sort x)
-  (step : (it : Iter (α := α) m β) →
-    (ih_yield : ∀ {it' : Iter (α := α) m β} {out : β}, it.plausible_step (.yield it' out) → motive it') →
-    (ih_skip : ∀ {it' : Iter (α := α) m β}, it.plausible_step (.skip it') → motive it' ) →
-    motive it) (it : Iter (α := α) m β) : motive it :=
-  step _ (fun {it' _} _ => Iter.induct motive step it') (fun {it'} _ => Iter.induct motive step it')
+def IterM.induct {α m β} [Iterator α m β] [Finite α m]
+  (motive : IterM (α := α) m β → Sort x)
+  (step : (it : IterM (α := α) m β) →
+    (ih_yield : ∀ {it' : IterM (α := α) m β} {out : β}, it.plausible_step (.yield it' out) → motive it') →
+    (ih_skip : ∀ {it' : IterM (α := α) m β}, it.plausible_step (.skip it') → motive it' ) →
+    motive it) (it : IterM (α := α) m β) : motive it :=
+  step _ (fun {it' _} _ => IterM.induct motive step it') (fun {it'} _ => IterM.induct motive step it')
 termination_by it.finitelyManySteps
 
-theorem Iter.DefaultConsumers.toArrayMapped.go.aux₁ [Monad m] [LawfulMonad m] [Iterator α m β] [Finite α m]
-    {it : Iter (α := α) m β} {b : γ} {bs : Array γ} {f : β → m γ} :
-    Iter.DefaultConsumers.toArrayMapped.go f it (#[b] ++ bs) = (#[b] ++ ·) <$> Iter.DefaultConsumers.toArrayMapped.go f it bs := by
-  induction it, bs using Iter.DefaultConsumers.toArrayMapped.go.induct
+theorem IterM.DefaultConsumers.toArrayMapped.go.aux₁ [Monad m] [LawfulMonad m] [Iterator α m β] [Finite α m]
+    {it : IterM (α := α) m β} {b : γ} {bs : Array γ} {f : β → m γ} :
+    IterM.DefaultConsumers.toArrayMapped.go f it (#[b] ++ bs) = (#[b] ++ ·) <$> IterM.DefaultConsumers.toArrayMapped.go f it bs := by
+  induction it, bs using IterM.DefaultConsumers.toArrayMapped.go.induct
   next it bs ih₁ ih₂ =>
   rw [go, map_eq_pure_bind, go, bind_assoc]
-  refine congrArg (Iter.stepH it >>= ·) ?_
+  refine congrArg (IterM.stepH it >>= ·) ?_
   ext step
   generalize step.inflate = step
   split
@@ -28,120 +28,120 @@ theorem Iter.DefaultConsumers.toArrayMapped.go.aux₁ [Monad m] [LawfulMonad m] 
   · simp [ih₂ _ ‹_›]
   · simp
 
-theorem Iter.DefaultConsumers.toArrayMapped.go.aux₂ [Monad m] [LawfulMonad m]
-    [Iterator α m β] [Finite α m] {it : Iter (α := α) m β} {acc : Array γ} {f : β → m γ} :
-    Iter.DefaultConsumers.toArrayMapped.go f it acc =
-      (acc ++ ·) <$> Iter.DefaultConsumers.toArrayMapped f it := by
+theorem IterM.DefaultConsumers.toArrayMapped.go.aux₂ [Monad m] [LawfulMonad m]
+    [Iterator α m β] [Finite α m] {it : IterM (α := α) m β} {acc : Array γ} {f : β → m γ} :
+    IterM.DefaultConsumers.toArrayMapped.go f it acc =
+      (acc ++ ·) <$> IterM.DefaultConsumers.toArrayMapped f it := by
   rw [← Array.toArray_toList (xs := acc)]
   generalize acc.toList = acc
   induction acc with
   | nil => simp [toArrayMapped]
   | cons x xs ih =>
-    rw [List.toArray_cons, Iter.DefaultConsumers.toArrayMapped.go.aux₁, ih]
+    rw [List.toArray_cons, IterM.DefaultConsumers.toArrayMapped.go.aux₁, ih]
     simp only [Functor.map_map, Array.append_assoc]
 
-theorem Iter.DefaultConsumers.toArrayMapped_of_stepH [Monad m] [LawfulMonad m]
-    [Iterator α m β] [Finite α m] {it : Iter (α := α) m β} {f : β → m γ} :
-    Iter.DefaultConsumers.toArrayMapped f it = (do
+theorem IterM.DefaultConsumers.toArrayMapped_of_stepH [Monad m] [LawfulMonad m]
+    [Iterator α m β] [Finite α m] {it : IterM (α := α) m β} {f : β → m γ} :
+    IterM.DefaultConsumers.toArrayMapped f it = (do
       match (← it.stepH).inflate with
-      | .yield it' out _ => return #[← f out] ++ (← Iter.DefaultConsumers.toArrayMapped f it')
-      | .skip it' _ => Iter.DefaultConsumers.toArrayMapped f it'
+      | .yield it' out _ => return #[← f out] ++ (← IterM.DefaultConsumers.toArrayMapped f it')
+      | .skip it' _ => IterM.DefaultConsumers.toArrayMapped f it'
       | .done _ => return #[]) := by
-  rw [Iter.DefaultConsumers.toArrayMapped, Iter.DefaultConsumers.toArrayMapped.go]
+  rw [IterM.DefaultConsumers.toArrayMapped, IterM.DefaultConsumers.toArrayMapped.go]
   apply bind_congr
   intro step
   generalize step.inflate = step
-  split <;> simp [Iter.DefaultConsumers.toArrayMapped.go.aux₂]
+  split <;> simp [IterM.DefaultConsumers.toArrayMapped.go.aux₂]
 
-theorem Iter.DefaultConsumers.toArrayMapped_of_step [Monad m] [LawfulMonad m]
-    [Iterator α m β] [Finite α m] {it : Iter (α := α) m β} {f : β → m γ} :
-    Iter.DefaultConsumers.toArrayMapped f it = (do
+theorem IterM.DefaultConsumers.toArrayMapped_of_step [Monad m] [LawfulMonad m]
+    [Iterator α m β] [Finite α m] {it : IterM (α := α) m β} {f : β → m γ} :
+    IterM.DefaultConsumers.toArrayMapped f it = (do
       match ← it.step with
-      | .yield it' out _ => return #[← f out] ++ (← Iter.DefaultConsumers.toArrayMapped f it')
-      | .skip it' _ => Iter.DefaultConsumers.toArrayMapped f it'
+      | .yield it' out _ => return #[← f out] ++ (← IterM.DefaultConsumers.toArrayMapped f it')
+      | .skip it' _ => IterM.DefaultConsumers.toArrayMapped f it'
       | .done _ => return #[]) := by
-  rw [Iter.DefaultConsumers.toArrayMapped_of_stepH, Iter.step, map_eq_pure_bind, bind_assoc]
+  rw [IterM.DefaultConsumers.toArrayMapped_of_stepH, IterM.step, map_eq_pure_bind, bind_assoc]
   apply bind_congr
   intro step
   generalize step.inflate = step
   rw [pure_bind]
   rfl
 
-theorem Iter.toArray_of_step [Monad m] [LawfulMonad m]
+theorem IterM.toArray_of_step [Monad m] [LawfulMonad m]
     [Iterator α m β] [IteratorToArray α m] [LawfulIteratorToArray α m]
-    {it : Iter (α := α) m β} :
+    {it : IterM (α := α) m β} :
     it.toArray = (do
       match ← it.step with
       | .yield it' out _ => return #[out] ++ (← it'.toArray)
       | .skip it' _ => it'.toArray
       | .done _ => return #[]) := by
-  rw [Iter.toArray, LawfulIteratorToArray.lawful, Iter.DefaultConsumers.toArrayMapped_of_step]
+  rw [IterM.toArray, LawfulIteratorToArray.lawful, IterM.DefaultConsumers.toArrayMapped_of_step]
   simp only [bind_pure_comp, pure_bind, toArray, LawfulIteratorToArray.lawful]
 
-theorem Iter.toList_toArray [Monad m] [Iterator α m β] [IteratorToArray α m]
-    {it : Iter (α := α) m β} :
+theorem IterM.toList_toArray [Monad m] [Iterator α m β] [IteratorToArray α m]
+    {it : IterM (α := α) m β} :
     Array.toList <$> it.toArray = it.toList := by
-  simp [Iter.toList]
+  simp [IterM.toList]
 
-theorem Iter.toArray_toList [Monad m] [LawfulMonad m] [Iterator α m β] [IteratorToArray α m]
-    {it : Iter (α := α) m β} :
+theorem IterM.toArray_toList [Monad m] [LawfulMonad m] [Iterator α m β] [IteratorToArray α m]
+    {it : IterM (α := α) m β} :
     List.toArray <$> it.toList = it.toArray := by
-  simp [Iter.toList]
+  simp [IterM.toList]
 
-theorem Iter.toList_of_step [Monad m] [LawfulMonad m] [Iterator α m β]
-    [IteratorToArray α m] [LawfulIteratorToArray α m] {it : Iter (α := α) m β} :
+theorem IterM.toList_of_step [Monad m] [LawfulMonad m] [Iterator α m β]
+    [IteratorToArray α m] [LawfulIteratorToArray α m] {it : IterM (α := α) m β} :
     it.toList = (do
       match ← it.step with
       | .yield it' out _ => return out :: (← it'.toList)
       | .skip it' _ => it'.toList
       | .done _ => return []) := by
-  simp [← Iter.toList_toArray]
-  rw [Iter.toArray_of_step, map_eq_pure_bind, bind_assoc]
+  simp [← IterM.toList_toArray]
+  rw [IterM.toArray_of_step, map_eq_pure_bind, bind_assoc]
   refine congrArg (_ >>= ·) ?_
   ext step
   split <;> simp
 
-theorem Iter.reverseToList.go.aux₁ [Monad m] [LawfulMonad m] [Iterator α m β] [Finite α m]
-    {it : Iter (α := α) m β} {b : β} {bs : List β} :
-    Iter.reverseToList.go it (bs ++ [b]) = (· ++ [b]) <$> Iter.reverseToList.go it bs:= by
-  induction it, bs using Iter.reverseToList.go.induct
+theorem IterM.reverseToList.go.aux₁ [Monad m] [LawfulMonad m] [Iterator α m β] [Finite α m]
+    {it : IterM (α := α) m β} {b : β} {bs : List β} :
+    IterM.reverseToList.go it (bs ++ [b]) = (· ++ [b]) <$> IterM.reverseToList.go it bs:= by
+  induction it, bs using IterM.reverseToList.go.induct
   next it bs ih₁ ih₂ =>
   rw [go, go, map_eq_pure_bind, bind_assoc]
-  refine congrArg (Iter.step it >>= ·) ?_
+  refine congrArg (IterM.step it >>= ·) ?_
   ext step
   simp only [List.cons_append] at ih₁
   split <;> simp [*]
 
-theorem Iter.reverseToList.go.aux₂ [Monad m] [LawfulMonad m] [Iterator α m β] [Finite α m]
-    {it : Iter (α := α) m β} {acc : List β} :
-    Iter.reverseToList.go it acc = (· ++ acc) <$> it.reverseToList := by
+theorem IterM.reverseToList.go.aux₂ [Monad m] [LawfulMonad m] [Iterator α m β] [Finite α m]
+    {it : IterM (α := α) m β} {acc : List β} :
+    IterM.reverseToList.go it acc = (· ++ acc) <$> it.reverseToList := by
   rw [← List.reverse_reverse (as := acc)]
   generalize acc.reverse = acc
   induction acc with
   | nil => simp [reverseToList]
-  | cons x xs ih => simp [Iter.reverseToList.go.aux₁, ih]
+  | cons x xs ih => simp [IterM.reverseToList.go.aux₁, ih]
 
-theorem Iter.reverseToList_of_step [Monad m] [LawfulMonad m] [Iterator α m β] [Finite α m]
-    {it : Iter (α := α) m β} :
+theorem IterM.reverseToList_of_step [Monad m] [LawfulMonad m] [Iterator α m β] [Finite α m]
+    {it : IterM (α := α) m β} :
     it.reverseToList = (do
       match ← it.step with
       | .yield it' out _ => return (← it'.reverseToList) ++ [out]
       | .skip it' _ => it'.reverseToList
       | .done _ => return []) := by
-  simp [Iter.reverseToList]
+  simp [IterM.reverseToList]
   rw [reverseToList.go]
   refine congrArg (it.step >>= ·) ?_
   ext step
   obtain ⟨step, h⟩ := step
-  cases step <;> simp [Iter.reverseToList.go.aux₂]
+  cases step <;> simp [IterM.reverseToList.go.aux₂]
 
 -- TODO: rename `reverseToList` -> `toListRev`
-theorem Iter.reverse_reverseToList [Monad m] [LawfulMonad m] [Iterator α m β]
+theorem IterM.reverse_reverseToList [Monad m] [LawfulMonad m] [Iterator α m β]
     [IteratorToArray α m] [LawfulIteratorToArray α m]
-    {it : Iter (α := α) m β} :
+    {it : IterM (α := α) m β} :
     List.reverse <$> it.reverseToList = it.toList := by
   apply Eq.symm
-  induction it using Iter.induct
+  induction it using IterM.induct
   rename_i it ihy ihs
   rw [reverseToList_of_step, toList_of_step, map_eq_pure_bind, bind_assoc]
   refine congrArg (_ >>= ·) ?_
@@ -152,17 +152,17 @@ end Consumers
 
 section Congruence
 
-theorem Iter.Morphism.toArrayMapped_eq {α α' : Type w} {m : Type w → Type w'}
+theorem IterM.Morphism.toArrayMapped_eq {α α' : Type w} {m : Type w → Type w'}
     {β : Type v} {γ : Type w}
     [Monad m] [LawfulMonad m]
     [Iterator α m β] [Iterator α' m β] [IteratorToArray α m] [LawfulIteratorToArray α m]
     [IteratorToArray α' m] [LawfulIteratorToArray α' m]
-    (φ : Morphism α α' m) {f : β → m γ} {it : Iter (α := α) m β} :
+    (φ : Morphism α α' m) {f : β → m γ} {it : IterM (α := α) m β} :
     IteratorToArray.toArrayMapped f it = IteratorToArray.toArrayMapped f (φ.map it) := by
   haveI : Finite α m := LawfulIteratorToArray.finite
   haveI : Finite α' m := LawfulIteratorToArray.finite
   simp only [LawfulIteratorToArray.lawful]
-  induction it using Iter.induct with | step it ihy ihs =>
+  induction it using IterM.induct with | step it ihy ihs =>
   rw [DefaultConsumers.toArrayMapped_of_stepH, DefaultConsumers.toArrayMapped_of_stepH]
   simp only [← φ.stepH_hom, map_eq_pure_bind, bind_assoc]
   apply bind_congr
@@ -171,20 +171,20 @@ theorem Iter.Morphism.toArrayMapped_eq {α α' : Type w} {m : Type w → Type w'
   obtain ⟨step, _⟩ := step
   cases step <;> simp (discharger := assumption) [PlausibilityMorphism.mapStep, IterStep.map, ihs, ihy]
 
-theorem Iter.Morphism.toArray_eq {α α' : Type w} {m : Type w → Type w'} {β : Type w}
+theorem IterM.Morphism.toArray_eq {α α' : Type w} {m : Type w → Type w'} {β : Type w}
     [Monad m] [LawfulMonad m]
     [Iterator α m β] [Iterator α' m β] [IteratorToArray α m] [LawfulIteratorToArray α m]
     [IteratorToArray α' m] [LawfulIteratorToArray α' m]
-    (φ : Morphism α α' m) {it : Iter (α := α) m β} :
+    (φ : Morphism α α' m) {it : IterM (α := α) m β} :
     it.toArray = (φ.map it).toArray := by
-  simp [Iter.toArray, φ.toArrayMapped_eq]
+  simp [IterM.toArray, φ.toArrayMapped_eq]
 
-theorem Iter.Morphism.toList_eq {α α' : Type w} {m : Type w → Type w'} {β : Type w}
+theorem IterM.Morphism.toList_eq {α α' : Type w} {m : Type w → Type w'} {β : Type w}
     [Monad m] [LawfulMonad m]
     [Iterator α m β] [Iterator α' m β] [IteratorToArray α m] [LawfulIteratorToArray α m]
     [IteratorToArray α' m] [LawfulIteratorToArray α' m]
-    (φ : Morphism α α' m) {it : Iter (α := α) m β} :
+    (φ : Morphism α α' m) {it : IterM (α := α) m β} :
     it.toList = (φ.map it).toList := by
-  simp [← Iter.toList_toArray, φ.toArray_eq]
+  simp [← IterM.toList_toArray, φ.toArray_eq]
 
 end Congruence
