Iterator/Consumers/Loop.lean
@@ -1,39 +1,39 @@
 import Iterator.Basic
 
-def Iter.ForInWillTerminate (α : Type w) (m : Type w → Type w') {β : Type v} [Iterator α m β] {γ : Type w}
+def IterM.ForInWillTerminate (α : Type w) (m : Type w → Type w') {β : Type v} [Iterator α m β] {γ : Type w}
     (successor_of : β → γ → γ → Prop) : Prop :=
-  WellFounded (fun (c' c : Iter (α := α) m β × γ) =>
+  WellFounded (fun (c' c : IterM (α := α) m β × γ) =>
     (c'.1.plausible_skip_successor_of c.1 ∧ c'.2 = c.2) ∨ (∃ b, c.1.plausible_step (.yield c'.1 b) ∧ successor_of b c.2 c'.2))
 
-def Iter.TerminationMeasures.ForInTerminates {α : Type w} {m : Type w → Type w'} {β : Type v} [Iterator α m β] {γ : Type w}
-    {successor_of : β → γ → γ → Prop} (_terminates : Iter.ForInWillTerminate α m successor_of) := Iter (α := α) m β × γ
+def IterM.TerminationMeasures.ForInTerminates {α : Type w} {m : Type w → Type w'} {β : Type v} [Iterator α m β] {γ : Type w}
+    {successor_of : β → γ → γ → Prop} (_terminates : IterM.ForInWillTerminate α m successor_of) := IterM (α := α) m β × γ
 
-def Iter.TerminationMeasures.ForInTerminates.mk {α : Type w} {m : Type w → Type w'} {β : Type v} [Iterator α m β] {γ : Type w}
-    {successor_of : β → γ → γ → Prop} (terminates : Iter.ForInWillTerminate α m successor_of) (it : Iter (α := α) m β) (c : γ) :
+def IterM.TerminationMeasures.ForInTerminates.mk {α : Type w} {m : Type w → Type w'} {β : Type v} [Iterator α m β] {γ : Type w}
+    {successor_of : β → γ → γ → Prop} (terminates : IterM.ForInWillTerminate α m successor_of) (it : IterM (α := α) m β) (c : γ) :
     ForInTerminates terminates :=
   (it, c)
 
 instance {α : Type w} {m : Type w → Type w'} {β : Type v} [Iterator α m β] {γ : Type w}
-    {successor_of : β → γ → γ → Prop} {terminates : Iter.ForInWillTerminate α m successor_of} :
-    WellFoundedRelation (Iter.TerminationMeasures.ForInTerminates terminates) where
+    {successor_of : β → γ → γ → Prop} {terminates : IterM.ForInWillTerminate α m successor_of} :
+    WellFoundedRelation (IterM.TerminationMeasures.ForInTerminates terminates) where
   rel p' p := (p'.1.plausible_skip_successor_of p.1 ∧ p'.2 = p.2) ∨ (∃ b, p.1.plausible_step (.yield p'.1 b) ∧ successor_of b p.2 p'.2)
   wf := terminates
 
 @[specialize]
-def Iter.DefaultConsumers.forIn {m : Type w → Type w'} {n : Type w → Type w''} [Monad n] [MonadLiftT m n]
+def IterM.DefaultConsumers.forIn {m : Type w → Type w'} {n : Type w → Type w''} [Monad n] [MonadLiftT m n]
     {α : Type w} {β : Type v} {γ : Type w}
     [Iterator α m β]
-    (it : Iter (α := α) m β) (init : γ) {successor_of : β → γ → γ → Prop}
+    (it : IterM (α := α) m β) (init : γ) {successor_of : β → γ → γ → Prop}
     (f : (b : β) → (c : γ) → n (Subtype fun s : ForInStep γ => successor_of b c s.value))
-    (terminates : Iter.ForInWillTerminate α m successor_of) : n γ := do
+    (terminates : IterM.ForInWillTerminate α m successor_of) : n γ := do
   match (← it.stepH).inflate with
   | .yield it' out _ =>
     match ← f out init with
-    | ⟨.yield c, _⟩ => Iter.DefaultConsumers.forIn it' c f terminates
+    | ⟨.yield c, _⟩ => IterM.DefaultConsumers.forIn it' c f terminates
     | ⟨.done c, _⟩ => return c
-  | .skip it' _ => Iter.DefaultConsumers.forIn it' init f terminates
+  | .skip it' _ => IterM.DefaultConsumers.forIn it' init f terminates
   | .done _ => return init
-termination_by Iter.TerminationMeasures.ForInTerminates.mk terminates it init
+termination_by IterM.TerminationMeasures.ForInTerminates.mk terminates it init
 decreasing_by
   · apply Or.inr
     exact ⟨out, ‹_›, ‹_›⟩
@@ -41,18 +41,18 @@ decreasing_by
     exact ⟨‹_›, rfl⟩
 
 class IteratorFor (α : Type w) (m : Type w → Type w') {β : Type v} [Iterator α m β] (n : Type w → Type w'') where
-  forIn : ∀ {γ : Type w}, Iter (α := α) m β → γ → {successor_of : β → γ → γ → Prop} →
+  forIn : ∀ {γ : Type w}, IterM (α := α) m β → γ → {successor_of : β → γ → γ → Prop} →
       ((b : β) → (c : γ) → n (Subtype fun s : ForInStep γ => successor_of b c s.value)) →
-      (Iter.ForInWillTerminate α m successor_of) → n γ
+      (IterM.ForInWillTerminate α m successor_of) → n γ
 
 class LawfulIteratorFor (α : Type w) (m : Type w → Type w') (n : Type w → Type w'')
     [Monad n] [Iterator α m β] [IteratorFor α m n] [MonadLiftT m n] where
   lawful : ∀ γ, IteratorFor.forIn (α := α) (m := m) (n := n) (γ := γ) =
-    Iter.DefaultConsumers.forIn (α := α) (m := m) (n := n) (γ := γ)
+    IterM.DefaultConsumers.forIn (α := α) (m := m) (n := n) (γ := γ)
 
 def IteratorFor.defaultImplementation {α : Type w} {m : Type w → Type w'} {n : Type w → Type w'}
     [Monad m] [Monad n] [MonadLiftT m n] [Iterator α m β] : IteratorFor α m n where
-  forIn := Iter.DefaultConsumers.forIn
+  forIn := IterM.DefaultConsumers.forIn
 
 instance (α : Type w) (m : Type w → Type w') (n : Type w → Type w')
     [Monad m] [Monad n] [MonadLiftT m n] [Iterator α m β] :
@@ -63,32 +63,32 @@ instance (α : Type w) (m : Type w → Type w') (n : Type w → Type w')
 
 instance {m : Type w → Type w'} {n : Type w → Type w''}
     {α : Type w} {β : Type v} [Iterator α m β] [Finite α m] [IteratorFor α m n] :
-    ForIn n (Iter (α := α) m β) β where
+    ForIn n (IterM (α := α) m β) β where
   forIn it init stepper := by
     apply IteratorFor.forIn it init (successor_of := fun _ _ _ => True) (fun b c => (⟨·, True.intro⟩) <$> stepper b c)
-    simp only [Iter.ForInWillTerminate]
-    refine Subrelation.wf (r := InvImage Iter.TerminationMeasures.Finite.rel (fun p => p.1.finitelyManySteps)) ?_ ?_
+    simp only [IterM.ForInWillTerminate]
+    refine Subrelation.wf (r := InvImage IterM.TerminationMeasures.Finite.rel (fun p => p.1.finitelyManySteps)) ?_ ?_
     · intro p' p h
       cases h
-      · apply Iter.TerminationMeasures.Finite.rel_of_skip
+      · apply IterM.TerminationMeasures.Finite.rel_of_skip
         rename_i h
         exact h.1
       · rename_i h
         obtain ⟨out, h, _⟩ := h -- Interesting: Moving `obtain` after `apply` leads to failure
-        apply Iter.TerminationMeasures.Finite.rel_of_yield
+        apply IterM.TerminationMeasures.Finite.rel_of_yield
         exact h
     · apply InvImage.wf
       exact WellFoundedRelation.wf
 
 @[specialize]
-def Iter.foldM {m : Type w → Type w'} {n : Type w → Type w'} [Monad n]
+def IterM.foldM {m : Type w → Type w'} {n : Type w → Type w'} [Monad n]
     {α : Type w} {β : Type v} {γ : Type w} [Iterator α m β] [Finite α m] [IteratorFor α m n]
-    (f : γ → β → n γ) (init : γ) (it : Iter (α := α) m β) : n γ :=
+    (f : γ → β → n γ) (init : γ) (it : IterM (α := α) m β) : n γ :=
   ForIn.forIn it init (fun x acc => ForInStep.yield <$> f acc x)
 
 @[specialize]
-def Iter.count {α : Type u} {β : Type v} [Iterator α Id β] [Finite α Id]
-    (it : Iter (α := α) Id β) : Nat :=
+def IterM.count {α : Type u} {β : Type v} [Iterator α Id β] [Finite α Id]
+    (it : IterM (α := α) Id β) : Nat :=
   go it 0
 where
   go [Finite α Id] it acc :=
@@ -99,8 +99,8 @@ where
   termination_by it.finitelyManySteps
 
 @[specialize]
-def Iter.countM {m : Type → Type w'} [Monad m] {α : Type} {β : Type v} [Iterator α m β] [Finite α m]
-    (it : Iter (α := α) m β) : m Nat :=
+def IterM.countM {m : Type → Type w'} [Monad m] {α : Type} {β : Type v} [Iterator α m β] [Finite α m]
+    (it : IterM (α := α) m β) : m Nat :=
   go it 0
 where
   go [Finite α m] it acc := do
@@ -111,7 +111,7 @@ where
   termination_by it.finitelyManySteps
 
 @[specialize]
-def Iter.drain {α : Type w} {m : Type w → Type w'} [Monad m] {β : Type v}
-    [Iterator α m β] [Finite α m] (it : Iter (α := α) m β) [IteratorFor α m m] :
+def IterM.drain {α : Type w} {m : Type w → Type w'} [Monad m] {β : Type v}
+    [Iterator α m β] [Finite α m] (it : IterM (α := α) m β) [IteratorFor α m m] :
     m PUnit :=
   it.foldM (γ := PUnit) (fun _ _ => pure .unit) .unit
