Iterator/Pure/Basic.lean
@@ -1,0 +1,10 @@
+import Iterator.Basic
+
+structure Iter {α : Type w} (β : Type v) : Type w where
+  inner : α
+
+def Iter.toIterM {α : Type w} {β : Type v} (it : Iter (α := α) β) : IterM (α := α) Id β :=
+  ⟨it.inner⟩
+
+def IterM.toPureIter {α : Type w} {β : Type v} (it : IterM (α := α) Id β) : Iter (α := α) β :=
+  ⟨it.inner⟩
